Work on TL proof.

LeanLTL/Examples/TrafficLights.lean
@@ -39,11 +39,14 @@ abbrev max_departs : LeanLTL.TraceFun ExState ℚ := LLTL[1]
 -- abbrev TL_Queues : {q | q=TL1_Q ∨ q=TL2_Q}
 
 -- Base Properties
-abbrev TL1GreenRedIff  := LLTL[G (TL1Green ↔ (¬TL1Red))]
-abbrev TL2GreenRedIff  := LLTL[G (TL2Green ↔ (¬TL2Red))]
+abbrev TL1StartGreen    := LLTL[TL1Green]
+abbrev TL2StartRed      := LLTL[TL2Red]
 
-abbrev TL1GreenNext     := LLTL[G ((TL1Green ∧ (TL1Queue == 0)) → (Xʷ (TL1Red ∧ TL2Green)))]
-abbrev TL2GreenNext     := LLTL[G ((TL2Green ∧ (TL2Queue == 0)) → (Xʷ (TL2Red ∧ TL1Green)))]
+abbrev TL1GreenRedIff   := LLTL[G (TL1Green ↔ (¬TL1Red))]
+abbrev TL2GreenRedIff   := LLTL[G (TL2Green ↔ (¬TL2Red))]
+
+abbrev TL1ToTL2Green    := LLTL[G ((TL1Green ∧ (TL1Queue == 0)) ↔ ((TL2Red ∧ TL1Green) ∧ (Xʷ (TL1Red ∧ TL2Green))))]
+abbrev TL2ToTL1Green    := LLTL[G ((TL2Green ∧ (TL2Queue == 0)) ↔ ((TL1Red ∧ TL2Green) ∧ (Xʷ (TL2Red ∧ TL1Green))))]
 
 abbrev TL1GreenDeparts  := LLTL[G (TL1Green → (TL1Departs == max_departs))]
 abbrev TL1RedDeparts    := LLTL[G (TL1Red → (TL1Departs == 0))]
@@ -56,9 +59,10 @@ abbrev TL2ArrivesBounds := LLTL[G (0 ≤ TL2Arrives ∧ TL2Arrives ≤ max_arriv
 abbrev TL1QueueNext     := LLTL[G ((X TL1Queue) == TL1Queue + TL1Arrives - TL1Departs)]
 abbrev TL2QueueNext     := LLTL[G ((X TL2Queue) == TL2Queue + TL2Arrives - TL2Departs)]
 
-abbrev TLBaseProperties := LLTL[TL1GreenRedIff ∧ TL2GreenRedIff ∧ TL1GreenNext ∧ TL2GreenNext
-                            ∧ TL1GreenDeparts ∧ TL1RedDeparts ∧ TL2GreenDeparts ∧ TL2RedDeparts
-                            ∧ TL1ArrivesBounds ∧ TL2ArrivesBounds ∧ TL1QueueNext ∧ TL2QueueNext]
+abbrev TLBaseProperties := LLTL[TL1StartGreen ∧ TL2StartRed ∧ TL1GreenRedIff ∧ TL2GreenRedIff
+                            ∧ TL1ToTL2Green ∧ TL2ToTL1Green ∧ TL1GreenDeparts ∧ TL1RedDeparts
+                            ∧ TL2GreenDeparts ∧ TL2RedDeparts ∧ TL1ArrivesBounds ∧ TL2ArrivesBounds
+                            ∧ TL1QueueNext ∧ TL2QueueNext]
 
 
 -- Optional Properties
@@ -68,12 +72,46 @@ abbrev TrafficLulls       := LLTL[(G (F (TL1Arrives == 0))) ∧ (G (F (TL2Arrive
 
 
 -- Goal Properties
-abbrev LightSafety        := LLTL[G ((TL1Green → ¬TL2Green) ∧ (TL2Green → ¬TL1Green))]
+abbrev LightSafety        := LLTL[G (TL1Green ↔ ¬TL2Green)]
 abbrev NeverStarvation    := LLTL[(G (F (TL1Queue == 0))) ∧ (G (F (TL2Queue == 0)))]
 
 
 -- Example Proofs
-theorem SatisfiesLightSafety : TLBaseProperties ⇒ LightSafety := sorry
+theorem SatisfiesLightSafety : TLBaseProperties ⇒ LightSafety := by
+  simp [TLBaseProperties, LeanLTL.TraceSet.sem_imp_iff, LeanLTL.TraceSet.sat_imp_iff]
+  intro t h
+  simp [LeanLTL.TraceSet.sat_and_iff] at h
+  rcases h with ⟨h1, h2, h3, h4, h5, h6, h7, h8, h9, h10, h11, h12, h13, h14⟩
+  simp [LightSafety]
+
+  apply LeanLTL.TraceSet.globally_induction
+  . simp_all [push_fltl]
+    by_contra; rename_i contra
+    specialize h4 0 (by simp)
+    simp_all
+  . simp [push_fltl]
+    intro n h_n h15 h_n_1
+    simp [push_fltl] at *
+    by_cases h_last_state: t.shift n h_n ⊨ TL1Green
+    . have h15 := h15.mp h_last_state
+      simp [*] at h15
+      specialize h5 n h_n
+      by_cases h_switch: (t.shift n h_n)⊨LLTL[TL1Queue == 0]
+      . have := h5.mp
+        specialize this (by simp_all)
+        rcases this with ⟨h17, h18⟩
+        specialize h18 h_n_1
+        simp_all
+      . have : ¬(((t.shift n h_n ⊨ TL1Green) ∧ t.shift n h_n ⊨ TL1Queue.eq (LeanLTL.TraceFun.const 0))) := by simp_all
+        simp [this, h15, h_last_state, h_switch] at h5
+        simp_all
+        specialize h3 (1+n) sorry
+        specialize h4 (1+n) sorry
+
+        sorry
+
+      sorry
+    . sorry
 
 theorem NeverStarvationCase1 : LLTL[ArrivesLtDeparts ∧ TLBaseProperties] ⇒ NeverStarvation := sorry
 
